\documentclass[12pt]{article}
\input{customcommands}

%=============

\begin{document}
\title{MATH103 Combinatorics Notes}
\author{Xuehuai He}
\maketitle

\hypertarget{toc}{}
{\parskip=0.05in
\tableofcontents}

\spl

\newpage
\pagestyle{updated}
\section{Combinatorics}
\subsection{A1 Intro}
\rmk Let there be a set $\{1,2,\dots,n\}$. The number of subsets of it is $2^n$ since for each number, we could say ``include'' or ``exclude''.

\eg Now consider the number of subsets with no two adjacent elements. Call them \textit{good} subsets, and the count be $f(n)$.

\ontangent{

    First consider $n=0$. Then the only \textit{good} subset is $\emptyset$.
    
    Now consider $n=1$, both $\emptyset, \{1\}$ are good.

    Now consider $n=2$. We have subsets: $\emptyset, 1, 2, 12$\sidenote{notation simplified for fast typing}. The set 12 is not good.

    Similarly, we have $f(3)=5, f(5)=8$.

}

We have $f(n)=f(n-1)+f(n-2)$ for all $n\geq 2$. Hence, $f(n)$ is the sequence that satisfies the recurrence relation and the initial conditions $f(0)=1, f(1)=2$.

\subsection{A2 Fibonnacci Sequence}
\begin{align*}
    0,1,1,2,3,5,8,13,21,34,55,89,144,233,377,\dots
\end{align*}

\rmk Two notation conventions: \begin{itemize}
    \item $F_0=1, F_1=1, F_n=F_{n-1}+F_{n-2}\quad \forall n\geq 2$, and\sidenote{Textbook}
    \item $f_0=0, f_1=1, f_n=f_{n-1}+f_{n-2}\quad \forall n\geq 2$.\sidenote{Preferred!}
\end{itemize}

\begin{table}[htbp]
    \centering
    \caption{Table of the sequence in two notations}
    \begin{tabular}{cccccccccc}
        $n$   & 0& 1& 2& 3& 4& 5& 6& 7& 8\\
        $F_n$ & 1& 1& 2& 3& 5& 8& 13& 21& 34\\
        $f_n$ & 0& 1& 1& 2& 3& 5& 8& 13& 21
    \end{tabular}
\end{table}\sidenote{It is the same recurrence as A1 but with init conditions shifted: $f(n)=F_{n+1}=f_{n+2}$.}

\eg Prof Rad is climbing 47 steps. Energized by coffee, she sometimes climbds one step per stride, sometimes two steps per stride. In how many ways can she do this?

\ontangent{Let $S(n)$ be the number of ways climbing $n$ steps.
\begin{itemize}
    \parskip=0.2in
    \item $S(1)=1$\hfill {\begin{tikzcd}[ampersand replacement=\&,cramped,sep=small]
        \bullet \& \bullet
        \arrow[no head, from=1-1, to=1-2]
    \end{tikzcd}}
    \item $S(2)=2$\hfill \begin{tikzcd}[ampersand replacement=\&,cramped,column sep=small,row sep=tiny]
        \bullet \& \bullet \& \bullet \\
        \bullet \&\& \bullet
        \arrow[no head, from=1-1, to=1-2]
        \arrow[no head, from=1-2, to=1-3]
        \arrow[no head, from=2-1, to=2-3]
    \end{tikzcd}
    \item $S(3)=3$ \hfill \begin{tikzcd}[ampersand replacement=\&,cramped,column sep=small,row sep=tiny]
        \bullet \& \bullet \& \bullet \& \bullet \\
        \bullet \&\& \bullet \& \bullet \\
        \bullet \& \bullet \&\& \bullet
        \arrow[no head, from=1-1, to=1-2]
        \arrow[no head, from=1-2, to=1-3]
        \arrow[no head, from=2-1, to=2-3]
        \arrow[no head, from=1-3, to=1-4]
        \arrow[no head, from=2-3, to=2-4]
        \arrow[no head, from=3-1, to=3-2]
        \arrow[no head, from=3-2, to=3-4]
    \end{tikzcd}
    \item $S(4)=5$ \hfill \begin{tikzcd}[ampersand replacement=\&,cramped,column sep=small,row sep=tiny]
        \bullet \& \bullet \& \bullet \& \bullet \& \bullet \\
        \bullet \&\& \bullet \& \bullet \& \bullet \\
        \bullet \& \bullet \&\& \bullet \& \bullet \\
        \bullet \& \bullet \& \bullet \&\& \bullet \\
        \bullet \&\& \bullet \&\& \bullet
        \arrow[no head, from=1-1, to=1-2]
        \arrow[no head, from=1-2, to=1-3]
        \arrow[no head, from=2-1, to=2-3]
        \arrow[no head, from=1-3, to=1-4]
        \arrow[no head, from=2-3, to=2-4]
        \arrow[no head, from=3-1, to=3-2]
        \arrow[no head, from=3-2, to=3-4]
        \arrow[no head, from=1-4, to=1-5]
        \arrow[no head, from=2-4, to=2-5]
        \arrow[no head, from=3-4, to=3-5]
        \arrow[no head, from=4-1, to=4-2]
        \arrow[no head, from=4-2, to=4-3]
        \arrow[no head, from=4-3, to=4-5]
        \arrow[no head, from=5-1, to=5-3]
        \arrow[no head, from=5-3, to=5-5]
    \end{tikzcd}
\end{itemize}
Conjecture: maybe Fibonnacci?

}
\begin{proof}
    Consider the set of ways she can cover $n$ steps. We have two cases:\begin{enumerate}
        \item Her first stride is 1 step. Then, the number of ways is the number of ways to cover the remaining $n-1$ steps. Thus, this gives us $S(n-1)$ ways.
        \item Her first stride is 2 steps. Then the number of ways is the number of ways to cover the remaining $n-2$ steps. Thus, this gives us $S(n-2)$ ways.
    \end{enumerate}
    Therefore, we conclude that $S(n)=S(n-1)+S(n-2)$. We account the initial conditions and conclude the closed form: \begin{align*}
        S(n) = F_n = f_{n+1}
    \end{align*}
    for all $n$. Since Prof Rad climbs 47 steps, we get \circled{$S(47)=4807526976$}.
\end{proof}

\subsection{A3 Simplex numbers}
\defn \textit{Two-dimensional} triangular numbers: $T_2(n)=1+2+3+\dots+n$
\begin{itemize}
    \item $T_2(1)=1$\hfill \begin{tikzcd}[ampersand replacement=\&,cramped,sep=tiny]
        \bullet
    \end{tikzcd}
    \item $T_2(2)=1+2=3$\hfill \begin{tikzcd}[ampersand replacement=\&,cramped,sep=tiny]
        \& \bullet \\
        \bullet \& \bullet
        \arrow[no head, from=1-2, to=2-2]
        \arrow[no head, from=1-2, to=2-1]
        \arrow[no head, from=2-1, to=2-2]
    \end{tikzcd}
    \item \dots
\end{itemize}
\begin{align*}
    1,3,6,10,15,21,28,36,45,55,\dots
\end{align*}
\addlink{Triangular numbers}

\begin{theorem}
    $T_2(n)=1+2+\dots+n=\frac{n(n+1)}{2}$
\end{theorem}
\begin{proof}[First proof]We prove by induction.\sidenote{Not as good of a proof: we must know what we are proving in the first place!}
    \begin{itemize}[align=left]
        \item[Base case $n=1$:] $T_2(1)=1$, formula gives $\frac{1(1+1)}{2}=1$.
        \item[Inductive hypothesis:] Suppose proved formula for up to $n=k$.
        \item[Inductive step:] Consider $n=k+1$. \begin{align*}
            T_2(k+1)&=1+\dots+k+(k+1)\\
            &= T_2(k)+k+1\\
            &= \frac{k(k+1)}{2}+k+1\\
            &= \frac{k^2+k+2(k+1)}{2}\\
            &= \frac{k^2+3k+2}{2}\\
            &= \frac{(k+1)(k+2)}{2}\\
            &= \frac{(k+1)\left((k+1)+1\right)}{2}
        \end{align*}  
    \end{itemize}
\end{proof}

\begin{proof}[Proof by Gauss]
    Observe:\sidenote{Better proof: concluding the formula without knowing it first!}
    \begin{align*}
        T_2(n) & = 1+2 +\dots + (n-1) + n\\
        &= n+(n-1) + \dots + 2 + 1
    \end{align*}
    Therefore, we \textbf{add} the two rows:
    \begin{align*}
        2T_2(n)&= \underset{n}{\underbrace{(n+1)+(n+1)+\dots+(n+1)}}\\
        &= n(n+1)\\
        \therefore T_2(n) = \frac{1}{2}n(n+1)
    \end{align*}
\end{proof}

\defn Tetrahedral numbers: $T_3(n) = T_2(1) + T_2(2)+\dots + T_2(n)$
\begin{itemize}
    \item $T_3(5) = 1+3+6+10+15=35$
\end{itemize}
\addlink{Tetrahedral numbers}

\defn Simplex numbers: $T_{k+1}(n) = T_k(1) + \dots +T_k(n)$
\addlink{Simplex numbers}

\end{document} 
